src/Lean/Meta/Tactic/Grind/Arith/Cutsat.lean
@@ -13,7 +13,7 @@ import Lean.Meta.Tactic.Grind.Arith.Cutsat.Proof
 import Lean.Meta.Tactic.Grind.Arith.Cutsat.Types
 import Lean.Meta.Tactic.Grind.Arith.Cutsat.Util
 import Lean.Meta.Tactic.Grind.Arith.Cutsat.Var
-import Lean.Meta.Tactic.Grind.Arith.Cutsat.Eq
+import Lean.Meta.Tactic.Grind.Arith.Cutsat.EqCnstr
 
 namespace Lean
 
