src/Lean/Meta/Tactic/Grind/Arith/Cutsat/EqCnstr.lean
@@ -1,0 +1,66 @@
+/-
+Copyright (c) 2025 Amazon.com, Inc. or its affiliates. All Rights Reserved.
+Released under Apache 2.0 license as described in the file LICENSE.
+Authors: Leonardo de Moura
+-/
+prelude
+import Lean.Meta.Tactic.Grind.Arith.Cutsat.Var
+
+namespace Lean.Meta.Grind.Arith.Cutsat
+def mkEqCnstr (p : Poly) (h : EqCnstrProof) : GoalM EqCnstr := do
+  return { p, h, id := (← mkCnstrId) }
+
+@[export lean_process_cutsat_eq]
+def processNewEqImpl (a b : Expr) : GoalM Unit := do
+  trace[grind.cutsat.eq] "{mkIntEq a b}"
+  -- TODO
+  return ()
+
+@[export lean_process_new_cutsat_lit]
+def processNewEqLitImpl (a k : Expr) : GoalM Unit := do
+  trace[grind.cutsat.eq] "{mkIntEq a k}"
+  -- TODO
+  return ()
+
+/-- Different kinds of terms internalized by this module. -/
+private inductive SupportedTermKind where
+  | add | mul | num
+
+private def isForbiddenParent (parent? : Option Expr) (k : SupportedTermKind) : Bool := Id.run do
+  let some parent := parent? | return false
+  let .const declName _ := parent.getAppFn | return false
+  if declName == ``HAdd.hAdd || declName == ``LE.le || declName == ``Dvd.dvd then return true
+  match k with
+  | .add => return false
+  | .mul => return declName == ``HMul.hMul
+  | .num => return declName == ``HMul.hMul || declName == ``Eq
+
+private def internalizeCore (e : Expr) (parent? : Option Expr) (k : SupportedTermKind) : GoalM Unit := do
+  if (← get').terms.contains { expr := e } then return ()
+  if isForbiddenParent parent? k then return ()
+  let p ← toPoly e
+  markAsCutsatTerm e
+  trace[grind.cutsat.internalize] "{aquote e}:= {← p.pp}"
+  modify' fun s => { s with terms := s.terms.insert { expr := e } p }
+
+/--
+Internalizes an integer expression. Here are the different cases that are handled.
+
+- `a + b` when `parent?` is not `+`, `≤`, or `∣`
+- `k * a` when `k` is a numeral and `parent?` is not `+`, `*`, `≤`, `∣`
+- numerals when `parent?` is not `+`, `*`, `≤`, `∣`, `=`.
+  Recall that we must internalize numerals to make sure we can propagate equalities
+  back to the congruence closure module. Example: we have `f 5`, `f x`, `x - y = 3`, `y = 2`.
+-/
+def internalize (e : Expr) (parent? : Option Expr) : GoalM Unit := do
+  let k ← if (← isAdd e) then
+    pure .add
+  else if (← isMul e) then
+    pure .mul
+  else if (← getIntValue? e).isSome then
+    pure .num
+  else
+    return ()
+  internalizeCore e parent? k
+
+end Lean.Meta.Grind.Arith.Cutsat
