src/Lean/Meta/Tactic/Grind/Arith/Cutsat/Types.lean
@@ -13,6 +13,11 @@ namespace Lean.Meta.Grind.Arith.Cutsat
 
 export Int.Linear (Var Poly)
 
+/-
+Remark: we will not define a parent structure `Cnstr` with the common
+fields until the compiler provides support for avoiding the performance overhead.
+-/
+
 mutual
 /-- A divisibility constraint and its justification/proof. -/
 structure DvdCnstr where
@@ -29,6 +34,8 @@ inductive DvdCnstrProof where
   | solveCombine (c₁ c₂ : DvdCnstr)
   | solveElim (c₁ c₂ : DvdCnstr)
   | elim (c : DvdCnstr)
+  | ofEq (c : EqCnstr)
+  | subst (c₁ : EqCnstr) (c₂ : DvdCnstr)
 
 structure LeCnstr where
   p  : Poly
@@ -41,7 +48,18 @@ inductive LeCnstrProof where
   | norm (c : LeCnstr)
   | divCoeffs (c : LeCnstr)
   | combine (c₁ c₂ : LeCnstr)
+  | subst (c₁ : EqCnstr) (c₂ : LeCnstr)
   -- TODO: missing constructors
+
+structure EqCnstr where
+  p  : Poly
+  h  : EqCnstrProof
+  id : Nat
+
+inductive EqCnstrProof where
+  | expr (h : Expr)
+  | norm (c : EqCnstr)
+  | subst (c₁ : EqCnstr) (c₂ : EqCnstr)
 end
 
 /-- State of the cutsat procedure. -/
@@ -64,6 +82,27 @@ structure State where
   if `x` is the maximal variable in `c`, `c.isLe`, and `x` coefficient in `c` is positive.
   -/
   uppers : PArray (PArray LeCnstr) := {}
+  /--
+  Mapping from variable to equation constraint used to eliminate it. `solved` variables should not occur in
+  `dvdCnstrs`, `lowers`, or `uppers`.
+  -/
+  elimEqs : PArray (Option EqCnstr) := {}
+  /--
+  Elimination stack. For every variable in `elimStack`. If `x` in `elimStack`, then `elimEqs[x]` is not `none`.
+  -/
+  elimStack : List Var := []
+  /--
+  Mapping from terms (e.g., `x + 2*y + 2`, `3*x`, `5`) to polynomials representing them.
+  These are terms used to propagate equalities between this module and the congruence closure module.
+  -/
+  terms : PHashMap ENodeKey Poly := {}
+  /--
+  Mapping from variable to occurrences. For example, an entry `x ↦ {y, z}` means that `x` may occur in `dvdCnstrs`, `lowers`, or `uppers` of
+  variables `y` and `z`.
+  If `x` occurs in `dvdCnstrs[y]`, `lowers[y]`, or `uppers[y]`, then `y` is in `occurs[x]`, but the reverse is not true.
+  If `x` is in `elimStack`, then `occurs[x]` is the empty set.
+  -/
+  occurs : PArray (PHashSet Var) := {}
   /-- Partial assignment being constructed by cutsat. -/
   assignment : PArray Int := {}
   /-- Next unique id for a constraint. -/
