src/Lean/Meta/Tactic/Grind/Arith/Cutsat/Util.lean
@@ -50,6 +50,10 @@ def getVars : GoalM (PArray Expr) :=
 def getVar (x : Var) : GoalM Expr :=
   return (← get').vars[x]!
 
+/-- Returns `true` if `x` has been eliminated using an equality constraint. -/
+def eliminated (x : Var) : GoalM Bool :=
+  return (← get').elimEqs[x]!.isSome
+
 def mkCnstrId : GoalM Nat := do
   let id := (← get').nextCnstrId
   modify' fun s => { s with nextCnstrId := id + 1 }
@@ -65,35 +69,87 @@ private partial def shrink (a : PArray Int) (sz : Nat) : PArray Int :=
 def resetAssignmentFrom (x : Var) : GoalM Unit := do
   modify' fun s => { s with assignment := shrink s.assignment x }
 
-def DvdCnstr.isSorted (c : DvdCnstr) : Bool :=
-  c.p.isSorted
+def _root_.Int.Linear.Poly.pp (p : Poly) : GoalM MessageData := do
+  match p with
+  | .num k => return m!"{k}"
+  | .add 1 x p => go (quoteIfNotAtom (← getVar x)) p
+  | .add k x p => go m!"{k}*{quoteIfNotAtom (← getVar x)}" p
+where
+  go (r : MessageData)  (p : Int.Linear.Poly) : GoalM MessageData := do
+    match p with
+    | .num 0 => return r
+    | .num k => return m!"{r} + {k}"
+    | .add 1 x p => go m!"{r} + {quoteIfNotAtom (← getVar x)}" p
+    | .add k x p => go m!"{r} + {k}*{quoteIfNotAtom (← getVar x)}" p
+
+def _root_.Int.Linear.Poly.denoteExpr' (p : Poly) : GoalM Expr := do
+  let vars ← getVars
+  return (← p.denoteExpr (vars[·]!))
 
 def DvdCnstr.isTrivial (c : DvdCnstr) : Bool :=
   match c.p with
   | .num k' => k' % c.d == 0
   | _ => c.d == 1
 
+def DvdCnstr.pp (c : DvdCnstr) : GoalM MessageData := do
+  return m!"{c.d} ∣ {← c.p.pp}"
+
 def DvdCnstr.denoteExpr (c : DvdCnstr) : GoalM Expr := do
-  let vars ← getVars
-  return mkIntDvd (toExpr c.d) (← c.p.denoteExpr (vars[·]!))
+  return mkIntDvd (toExpr c.d) (← c.p.denoteExpr')
 
 def DvdCnstr.throwUnexpected (c : DvdCnstr) : GoalM α := do
-  throwError "`grind` internal error, unexpected{indentExpr (← c.denoteExpr)} "
-
-def LeCnstr.isSorted (c : LeCnstr) : Bool :=
-  c.p.isSorted
+  throwError "`grind` internal error, unexpected{indentD (← c.pp)} "
 
 def LeCnstr.isTrivial (c : LeCnstr) : Bool :=
   match c.p with
   | .num k => k ≤ 0
   | _ => false
 
+def LeCnstr.pp (c : LeCnstr) : GoalM MessageData := do
+  return m!"{← c.p.pp} ≤ 0"
+
 def LeCnstr.denoteExpr (c : LeCnstr) : GoalM Expr := do
-  let vars ← getVars
-  return mkIntLE (← c.p.denoteExpr (vars[·]!)) (mkIntLit 0)
+  return mkIntLE (← c.p.denoteExpr') (mkIntLit 0)
 
 def LeCnstr.throwUnexpected (c : LeCnstr) : GoalM α := do
-  throwError "`grind` internal error, unexpected{indentExpr (← c.denoteExpr)}"
+  throwError "`grind` internal error, unexpected{indentD (← c.pp)}"
+
+def EqCnstr.isTrivial (c : LeCnstr) : Bool :=
+  match c.p with
+  | .num k => k == 0
+  | _ => false
+
+def EqCnstr.pp (c : EqCnstr) : GoalM MessageData := do
+  return m!"{← c.p.pp} = 0"
+
+def EqCnstr.denoteExpr (c : EqCnstr) : GoalM Expr := do
+  return mkIntEq (← c.p.denoteExpr') (mkIntLit 0)
+
+def EqCnstr.throwUnexpected (c : LeCnstr) : GoalM α := do
+  throwError "`grind` internal error, unexpected{indentD (← c.pp)}"
+
+/-- Returns occurrences of `x`. -/
+def getOccursOf (x : Var) : GoalM (PHashSet Var) :=
+  return (← get').occurs[x]!
+
+/--
+Adds `y` as an occurrence of `x`.
+That is, `x` occurs in `lowers[y]`, `uppers[y]`, or `dvdCnstrs[y]`.
+-/
+def addOcc (x : Var) (y : Var) : GoalM Unit := do
+  unless (← getOccursOf x).contains y do
+    modify' fun s => { s with occurs := s.occurs.modify x fun ys => ys.insert y }
+
+/--
+Given `p` a polynomial being inserted into `lowers`, `uppers`, or `dvdCnstrs`,
+get its leading variable `y`, and adds `y` as an occurrence for the remaining variables in `p`.
+-/
+partial def _root_.Int.Linear.Poly.updateOccs (p : Poly) : GoalM Unit := do
+  let .add _ y p := p | throwError "`grind` internal error, unexpected constant polynomial"
+  let rec go (p : Poly) : GoalM Unit := do
+    let .add _ x p := p | return ()
+    addOcc x y; go p
+  go p
 
 def toContextExpr : GoalM Expr := do
   let vars ← getVars
