tests/lean/run/grind_pre.lean
@@ -1,5 +1,5 @@
 abbrev f (a : α) := a
-
+set_option grind.warning false
 set_option grind.debug true
 set_option grind.debug.proofs true
 
@@ -97,10 +97,10 @@ h_3 : ¬g (i + 1) j ⋯ = i + j + 1
   [offset] Assignment satisfying offset contraints
     [assign] j := 0
     [assign] i := 1
-    [assign] i + 1 := 2
-    [assign] 0 := 0
-    [assign] i + j + 1 := 1
-    [assign] i + j := 0
+    [assign] 「i + 1」 := 2
+    [assign] 「0」 := 0
+    [assign] 「i + j + 1」 := 1
+    [assign] 「i + j」 := 0
 -/
 #guard_msgs (error) in
 example (i j : Nat) (h : i + 1 > j + 1) : g (i+1) j = f ((fun x => x) i) + f j + 1 := by
